---
hide_table_of_contents: true
---
## 題目

+ (a) Prove the Lagrange's identity

    $$
    \bigg(\sum^n_{i=1}x_iy_i\bigg)^2 = \bigg(\sum^n_{i=1}x_i^2\bigg)\bigg(\sum^n_{i=1}y_i^2\bigg)-\sum_{1\leq i < j\leq n}(x_iy_j-x_jy_i)^2
    $$
    
    and use this to give another proof of the Cauchy-Schwarz inequality.

+ (b) Show that

    $$
    \bigg(\sum^n_{i=1}(x_i+y_i)^2\bigg)^{\frac{1}{2}}\leq\bigg(\sum^n_{i=1}x_i^2\bigg)^{\frac{1}{2}}+\bigg(\sum^n_{i=1}y_i^2\bigg)^{\frac{1}{2}}
    $$

## 解答

+ (a) Use induction is easily to fininsh. 

:::note 
[Cauchy-Schwarz inequality](https://en.wikipedia.org/wiki/Cauchy%E2%80%93Schwarz_inequality) is $\bigg(\sum^n_{i=1}x_iy_i\bigg)^2 \leq \bigg(\sum^n_{i=1}x_i^2\bigg)\bigg(\sum^n_{i=1}y_i^2\bigg)$
:::

+ (b)

    $$
    \begin{align*}
    \sqrt{\sum^n_{i=1}(x_i+y_i)^2}&=\sqrt{\sum^n_{i=1}x_i^2+\sum^n_{i=1}y_i^2+2\sum^n_{i=1}x_iy_i}\\
    &\leq\sqrt{\sum^n_{i=1}x_i^2+\sum^n_{i=1}y_i^2+2\sqrt{\bigg(\sum^n_{i=1}x_i^2\bigg)\bigg(\sum^n_{i=1}y_i^2\bigg)}}\\
    &=\sqrt{\sum^n_{i=1}x_i^2}+\sqrt{\sum^n_{i=1}y_i^2}
    \end{align*}
    $$