---
hide_table_of_contents: true
---
## 題目

If $\bm{A}^{m} = \bm{O}$ and $\bm{AB}=\bm{B}$, prove that $\bm{B}=\bm{O}$

## 解答

### 方法一

$$ 
\begin{align*}
\bm{B} = \bm{IB} &= \bm{(I-A^m)B}\\
&= \big(\sum\limits_{i=1}^{m}\bm{A^{m-i}}\big)\big(\bm{I-A}\big)\bm{B}\\
&= \big(\sum\limits_{i=1}^m \bm{A^{m-i}}\big)\big(\bm{B-AB}\big)\\
&= \bm{O}
\end{align*}
$$ 

### 方法二

$$ 
\begin{align*}
\bm{O} = \bm{OB} &= \bm{(A^m)B}\\
&= \big(\bm{A^{m-i}}\big)\big(\bm{AB}\big)\\
&= \big(\bm{A^{m-i}}\big)\big(\bm{B}\big)\\
&= \cdots\\
&= \bm{AB} = \bm{B}\\
\end{align*}
$$ 
