---
hide_table_of_contents: true
---
## 題目

If $\bm{A}$ is a skew-Hermitian, show that both $(\bm{I}-\bm{A})$ and $(\bm{I}+\bm{A})$ are invertible and that $\bm{C} = (\bm{I}-\bm{A})(\bm{I}+\bm{A})^{-1}$ is unitary.

## 解答

By [Sec 3.5 Q16](05_16) we have all eigenvalue of $\bm{A}$ are pure imaginary, then all eigenvalues of $\bm{I\pm A}$ are not zero, then both of them are invertible.

Since  

$$
\begin{align*}
\bm{C}^* &= \big({(\bm{I+A})}^{-1}\big)^*(\bm{I-A}^*)\\
&= \big({(\bm{I+A})}^*\big)^{-1}(\bm{I-A}^*)\\
&= {(\bm{I}+\bm{A}^*)}^{-1} (\bm{I+A})\\
&= (\bm{I-A})^{-1}(\bm{I+A})
\end{align*}
$$

and $(\bm{I-A})(\bm{I+A}) = \bm{I}-\bm{A}^2 = (\bm{I+A})(\bm{I-A})$.

Hence 

$$
\begin{align*}
\bm{C}^*\bm{C} &= (\bm{I-A})^{-1}(\bm{I+A})(\bm{I-A})(\bm{I+A})^{-1}\\
&= (\bm{I-A})^{-1}(\bm{I-A})(\bm{I+A})(\bm{I+A})^{-1}\\
& = \bm{I}
\end{align*}
$$